case_study/MinimalCaps/README.md
@@ -1,8 +1,34 @@
-# Cerise Comparison
+# MinimalCaps
+
+The MinimalCaps machine is a subset of CHERI-RISC-V, focusing on the capability
+related instructions and with some simplifications such as unbounded integers
+and no byte-addressing. The universal contract we prove is based on the Cerise
+work. At the end of this file we provide a paper-to-artifact correspondence.
+
+## How To Build
+
+This case study is part of the overall Katamaran build. When Katamaran is build,
+MinimalCaps will have been build as well. For instructions see: `README.md`.
+
+## Case Study Structure
+All files mentioned in this section are relative to `case_study/MinimalCaps/`.
+
+- `Base.v`: contains type declarations and hooks these into the appropriate Katamaran
+  modules.
+- `Machine.v`: contains the ISA specification in μSail. All functions are declared here,
+  as well as the foreign functions and signatures of the lemmas.
+- `Contracts.v`: contains the pure predicates, spatial predicate signatures and
+  user solver. Also contains the contract definitions and lemmas showing that
+  the defined contracts are valid. We also define contracts for foreign
+  functions and the lemmas of the case study (but these are proved in the `Model.v`).
+- `Model.v`: is the Iris part of the verification, we define an interpretation for each
+  spatial predicate and prove the soundness of the foreign functions and lemmas.
+- `LoopVerification.v`: is where the universal contract is proven, this happens over
+  the fdeCycle (i.e., the loop of the machine).
 
 ## Instructions
 
-| Cerise   | MinimalCaps (CHERI-RISC-V)                                                   |
+| Cerise   | MinimalCaps (⊆ CHERI-RISC-V)                                                 |
 |----------|------------------------------------------------------------------------------|
 | Fail     | Fail (“Illegal”1)                                                            |
 | Halt     | Ret (“HLT”2)                                                                 |
@@ -23,6 +49,20 @@
 | GetP     | CGetPerm(rd, cs)                                                             |
 | IsPtr    | CGetTag(rd, cs)                                                              |
 
-1: No literal “fail” instruction, but the effect can be achieved with any illegal instruction encoding (for example, writing “HLT” or “FAIL” as an instruction)
+## Paper-to-Artifact Correspondence
 
-2: The Ret of RISC-V will return from the subroutine, i.e., giving control back to the caller, an actual halt can be achieved similar to Fail
+| Paper                       | File                                        | Definition                           |
+|-----------------------------|---------------------------------------------|--------------------------------------|
+| Figure 4: Store instruction | `case_study/MinimalCaps/Machine.v`          | Definition fun_exec_sd               |
+| Figure 5: Capability safety | `case_study/MinimalCaps/Model.v`            | Definition interp                    |
+| Figure 6: UC Definition     | `case_study/MinimalCaps/LoopVerification.v` | Definition semContract_loop          |
+| Figure 6: UC Verif.         | `case_study/MinimalCaps/LoopVerification.v` | Lemma valid_semContract_loop2        |
+| Figure 10: Store contract   | `case_study/MinimalCaps/Contracts.v`        | Definition sep_contract_exec_sd      |
+| Figure 10: Store verif.     | `case_study/MinimalCaps/Contracts.v`        | Lemma valid_contract_exec_sd         |
+| Figure 11: read_mem         | `case_study/MinimalCaps/Contracts.v`        | Definition sep_contract_read_mem     |
+| Figure 11: read_reg         | `case_study/MinimalCaps/Contracts.v`        | Definition sep_contract_read_reg     |
+| Figure 11: read_reg_cap     | `case_study/MinimalCaps/Contracts.v`        | Definition sep_contract_read_reg_cap |
+| Figure 11: write_mem        | `case_study/MinimalCaps/Contracts.v`        | Definition sep_contract_write_mem    |
+| Figure 11: update_pc        | `case_study/MinimalCaps/Contracts.v`        | Definition sep_contract_update_pc    |
+| Figure 11: move_cursor      | `case_study/MinimalCaps/Contracts.v`        | Definition lemma_safe_move_cursor    |
+| Figure 11: subperm_not_E    | `case_study/MinimalCaps/Contracts.v`        | Definition lemma_subperm_not_E       |
